src/proof/string/prefix_suffix.v
@@ -1,6 +1,21 @@
 From New.proof Require Import prelude empty_ffi.
+From New.proof.string Require Export decimal.
 
 Section proof.
+
+Definition byte_dash : w8 := W8 45.  (* ASCII '-' *)
+Definition byte_slash : w8 := W8 47.  (* ASCII '/' *)
+
+Definition dash_free (s: go_string) : Prop :=
+  Forall (λ b, b ≠ byte_dash) s.
+
+Definition slash_free (s: go_string) : Prop :=
+  Forall (λ b, b ≠ byte_slash) s.
+
+Definition w8_eq_dec (x y : w8) : {x = y} + {x ≠ y}.
+Proof.
+  destruct (decide (x = y)); [left|right]; done.
+Defined.
 
 Lemma prefix_length_sep (sep : w8) prefix1 suffix1 prefix2 suffix2 :
   Forall (λ b, b ≠ sep) prefix1 →
@@ -17,7 +32,7 @@ Proof.
     apply app_eq_inv in Heq.
     destruct Heq as [(k & Hprefix_eq & Hsuffix_eq) | (k & Hprefix_eq & Hsuffix_eq)].
     + assert (k ≠ []) as Hk_nonempty.
-      { intros Hcontra. rewrite Hcontra in Hprefix_eq. rewrite app_nil_r in Hprefix_eq.
+      { intros Hcontra. rewrite Hcontra in Hprefix_eq. rewrite List.app_nil_r in Hprefix_eq.
         apply (f_equal length) in Hprefix_eq. lia. }
       destruct k as [|b k']; [done|].
       simpl in Hsuffix_eq. injection Hsuffix_eq as Hb_eq _.
@@ -27,7 +42,7 @@ Proof.
       apply Forall_cons_1 in Hk_no_sep.
       apply Hk_no_sep. reflexivity.
     + assert (k ≠ []) as Hk_nonempty.
-      { intros Hcontra. rewrite Hcontra in Hprefix_eq. rewrite app_nil_r in Hprefix_eq.
+      { intros Hcontra. rewrite Hcontra in Hprefix_eq. rewrite List.app_nil_r in Hprefix_eq.
         apply (f_equal length) in Hprefix_eq. lia. }
       destruct k as [|b k']; [done|].
       simpl in Hsuffix_eq. injection Hsuffix_eq as Hb_eq _.
@@ -36,61 +51,6 @@ Proof.
       apply Forall_app in Hno_sep2 as [_ Hk_no_sep].
       apply Forall_cons_1 in Hk_no_sep.
       apply Hk_no_sep. reflexivity.
-Qed.
-
-Lemma suffix_length_sep (sep : w8) prefix1 suffix1 prefix2 suffix2 :
-  Forall (λ b, b ≠ sep) suffix1 →
-    Forall (λ b, b ≠ sep) suffix2 →
-      prefix1 ++ [sep] ++ suffix1 = prefix2 ++ [sep] ++ suffix2 →
-        length prefix1 = length prefix2 ∧ length suffix1 = length suffix2.
-Proof.
-  intros Hno_sep1 Hno_sep2 Heq.
-  destruct (decide (length suffix1 = length suffix2)) as [Hlen_eq|Hneq].
-  - split; [|done].
-    apply (f_equal length) in Heq.
-    repeat rewrite app_length in Heq. simpl in Heq. lia.
-  - exfalso.
-    apply app_eq_inv in Heq.
-    destruct Heq as [(k & Hprefix_eq & Hsuffix_eq) | (k & Hprefix_eq & Hsuffix_eq)].
-    + assert (k ≠ []) as Hk_nonempty.
-      { intros Hcontra. rewrite Hcontra in Hsuffix_eq.
-        apply (f_equal length) in Hsuffix_eq.
-        simpl in Hsuffix_eq. lia. }
-      destruct k as [|b k']; [done|].
-      assert (b = sep) as Hb_sep.
-      { injection Hsuffix_eq as <- _. done. }
-      injection Hsuffix_eq as _ ->.
-      apply Forall_app in Hno_sep2 as [_ Hno_sep2_tail].
-      apply Forall_cons_1 in Hno_sep2_tail.
-      apply Hno_sep2_tail. reflexivity.
-    + assert (k ≠ []) as Hk_nonempty.
-      { intros Hcontra. rewrite Hcontra in Hsuffix_eq.
-        apply (f_equal length) in Hsuffix_eq.
-        simpl in Hsuffix_eq. lia. }
-      destruct k as [|b k']; [done|].
-      assert (b = sep) as Hb_sep.
-      { injection Hsuffix_eq as <- _. done. }
-      injection Hsuffix_eq as _ ->.
-      apply Forall_app in Hno_sep1 as [_ Hno_sep1_tail].
-      apply Forall_cons_1 in Hno_sep1_tail.
-      apply Hno_sep1_tail. reflexivity.
-Qed.
-
-Lemma app_sep_suffix_inj (sep: w8) prefix1 suffix1 prefix2 suffix2 :
-  Forall (λ b, b ≠ sep) suffix1 →
-    Forall (λ b, b ≠ sep) suffix2 →
-      prefix1 ++ [sep] ++ suffix1 = prefix2 ++ [sep] ++ suffix2 →
-        prefix1 = prefix2 ∧ suffix1 = suffix2.
-Proof.
-  intros Hno_sep1 Hno_sep2 Heq.
-  assert (length suffix1 = length suffix2) as Hlen_suffix.
-  { apply (suffix_length_sep sep _ _ _ _ Hno_sep1 Hno_sep2 Heq). }
-  assert (length ([sep] ++ suffix1) = length ([sep] ++ suffix2)) as Hlen'.
-  { simpl. lia. }
-  apply app_inj_2 in Heq; [|done].
-  destruct Heq as [Hprefix_eq Hsep_suffix_eq].
-  split; [done|].
-  injection Hsep_suffix_eq as ->. done.
 Qed.
 
 Lemma app_prefix_sep_inj (sep: w8) prefix1 suffix1 prefix2 suffix2 :
@@ -113,21 +73,33 @@ Proof.
   injection Hsep_suffix_eq as ->. done.
 Qed.
 
-Definition byte_dash : w8 := W8 45.  (* ASCII '-' *)
-Definition byte_slash : w8 := W8 47.  (* ASCII '/' *)
+Fixpoint strip_prefix (prefix s : go_string) : option go_string :=
+  match prefix, s with
+  | [], s => Some s
+  | p :: prefix, b :: s =>
+      if decide (p = b) then strip_prefix prefix s else None
+  | _ :: _, [] => None
+  end.
 
-Axiom reserved_name : go_string → Prop.
-
-Definition dash_free (s: go_string) : Prop :=
-  Forall (λ b, b ≠ byte_dash) s.
-
-Definition slash_free (s: go_string) : Prop :=
-  Forall (λ b, b ≠ byte_slash) s.
-
-Definition w8_eq_dec (x y : w8) : {x = y} + {x ≠ y}.
+Lemma strip_prefix_correct prefix s suffix :
+  strip_prefix prefix s = Some suffix →
+  s = prefix ++ suffix.
 Proof.
-  destruct (decide (x = y)); [left|right]; done.
-Defined.
+  revert s suffix.
+  induction prefix as [|p prefix IH]; intros s suffix Hstrip.
+  - simpl in Hstrip. by simplify_eq/=.
+  - destruct s as [|b s]; [done|].
+    simpl in Hstrip.
+    destruct (decide (p = b)) as [->|Hneq]; [|done].
+    rewrite (IH _ _ Hstrip). done.
+Qed.
+
+Lemma strip_prefix_complete prefix suffix :
+  strip_prefix prefix (prefix ++ suffix) = Some suffix.
+Proof.
+  induction prefix as [|p prefix IH]; simpl; [done|].
+  destruct (decide (p = p)); [done|congruence].
+Qed.
 
 Lemma slash_free_count_occ_zero s :
   slash_free s ↔ count_occ w8_eq_dec s byte_slash = 0%nat.
@@ -146,34 +118,6 @@ Proof.
       * discriminate.
       * constructor; [exact Hneq'|].
         apply IH. exact Hcount.
-Qed.
-
-Definition reserved_derived_name (derived_name: go_string) : Prop :=
-  ∃ prefix suffix,
-    reserved_name prefix ∧
-    dash_free suffix ∧
-    derived_name = prefix ++ "-"%go ++ suffix.
-
-Definition unreserved_generated_name (generated_name: go_string) : Prop :=
-    ∃ prefix suffix,
-      ¬ reserved_name prefix ∧
-      dash_free suffix ∧
-      length suffix = 5%nat ∧
-      generated_name = prefix ++ "-"%go ++ suffix.
-
-Lemma derived_name_and_generated_name_neq name1 name2 :
-  reserved_derived_name name1 →
-    unreserved_generated_name name2 →
-      name1 ≠ name2.
-Proof.
-  intros Hname1 Hname2 Hcontra.
-  destruct Hname1 as (prefix1 & suffix1 & Hreserved1 & Hdash_free1 & ->).
-  destruct Hname2 as (prefix2 & suffix2 & Hnotreserved2 & Hdash_free2 & Hlen2 & ->).
-  assert ("-"%go = [byte_dash]) as Hdash_eq by done.
-  rewrite Hdash_eq in Hcontra.
-  apply app_sep_suffix_inj in Hcontra; [|done|done].
-  destruct Hcontra as [-> _].
-  done.
 Qed.
 
 Lemma pod_controller_index_key_inj namespace1 kind1 name1 uid1 namespace2 kind2 name2 uid2 :
@@ -209,18 +153,6 @@ Proof.
   destruct Hns1_slash_free as [_ [Hcontra _]].
   apply Forall_cons_1 in Hcontra.
   apply Hcontra. reflexivity.
-Qed.
-
-Lemma pod_controller_index_key_inequality2 ns1 ns2 suffix1 suffix2 :
-  slash_free ns1 → slash_free ns2 → ns1 ≠ ns2 →
-  ns1 ++ "/"%go ++ suffix1 ≠ ns2 ++ "/"%go ++ suffix2.
-Proof.
-  intros Hns1_slash_free Hns2_slash_free Hns_neq Hcontra.
-  assert ("/"%go = [byte_slash]) as Hslash_eq by done.
-  rewrite Hslash_eq in Hcontra.
-  apply app_prefix_sep_inj in Hcontra; [|done|done].
-  destruct Hcontra as [Hns_eq _].
-  done.
 Qed.
 
 Lemma pod_controller_index_key_slash_count namespace kind name uid :
@@ -276,6 +208,5 @@ Proof.
   eapply pod_controller_index_key_inj; [|exact Heq].
   repeat split; eauto.
 Qed.
-
 
 End proof.
