src/proof/controllers/statefulset.v
@@ -1,0 +1,557 @@
+From New.proof Require Import prelude empty_ffi.
+From New.proof.string Require Export prefix_suffix.
+From New.proof.kubernetes_model Require Export get index create delete.
+From New.proof Require Export util.
+From New.proof.controllers Require Export common.
+From New.proof.controllers Require Export statefulset_init.
+From New.proof.k8s_io.kubernetes.pkg Require Export controller.
+From New.proof.k8s_io.apimachinery.pkg.runtime Require Export schema.
+From New.proof.k8s_io.apimachinery.pkg.api Require Export errors.
+
+Section proof.
+Context `{hG: !heapGS Σ}.
+Context {sem : go.Semantics}
+  {package_sem : code.controllers.statefulset.statefulset.Assumptions}.
+Collection W := sem + package_sem.
+#[local] Instance base_common_sem : common.Assumptions | 100 :=
+  code.controllers.statefulset.statefulset.import_common_Assumption.
+#[local] Instance controller_sem : controller.Assumptions :=
+  code.controllers.statefulset.statefulset.import_controller_Assumption.
+#[local] Instance runtime_sem : code.k8s_io.apimachinery.pkg.runtime.runtime.Assumptions :=
+  controller.import_runtime_Assumption.
+#[local] Instance base_apimodel_sem : apimodel.Assumptions | 100 :=
+  common.import_apimodel_Assumption.
+#[local] Instance object_meta_v1_sem :
+    code.k8s_io.apimachinery.pkg.apis.meta.v1.v1.Assumptions :=
+  apimodel.import_apis_meta_v1_Assumption.
+#[local] Instance object_apps_v1_sem :
+    code.k8s_io.api.apps.v1.v1.Assumptions :=
+  apimodel.import_api_apps_v1_Assumption.
+#[local] Instance object_core_v1_sem :
+    code.k8s_io.api.core.v1.v1.Assumptions :=
+  code.k8s_io.api.apps.v1.v1.import_core_v1_Assumption.
+#[local] Instance apimodel_sem : apimodel.Assumptions | 0.
+Proof using package_sem.
+  constructor; try exact object_core_v1_sem; try apply _.
+Defined.
+#[local] Instance common_sem : common.Assumptions | 0.
+Proof using package_sem.
+  constructor; try exact apimodel_sem; try apply _.
+Defined.
+Context `{!kubernetesModelG Σ}.
+Local Set Default Proof Using "All".
+
+Definition own_pod_frags γ dq (pod : PodV.t) : iProp Σ :=
+  own_meta_frag γ (PodV.key pod) pod.(PodV.ObjectMeta').(ObjectMetaV.UID') dq
+    pod.(PodV.ObjectMeta') ∗
+  own_spec_frag γ (PodV.key pod) pod.(PodV.ObjectMeta').(ObjectMetaV.UID') dq
+    (ObjectSpecV.PodSpec pod.(PodV.Spec')).
+
+Definition own_pods_frags γ dq (pods : list PodV.t) : iProp Σ :=
+  [∗ list] pod ∈ pods, own_pod_frags γ dq pod.
+
+Definition own_pvc_frags γ dq (pvc : PersistentVolumeClaimV.t) : iProp Σ :=
+  own_meta_frag γ (PersistentVolumeClaimV.key pvc)
+    pvc.(PersistentVolumeClaimV.ObjectMeta').(ObjectMetaV.UID') dq
+    pvc.(PersistentVolumeClaimV.ObjectMeta') ∗
+  own_spec_frag γ (PersistentVolumeClaimV.key pvc)
+    pvc.(PersistentVolumeClaimV.ObjectMeta').(ObjectMetaV.UID') dq
+    (ObjectSpecV.PersistentVolumeClaimSpec pvc.(PersistentVolumeClaimV.Spec')).
+
+Definition own_pvcs_frags γ dq (pvcs : list PersistentVolumeClaimV.t) : iProp Σ :=
+  [∗ list] pvc ∈ pvcs, own_pvc_frags γ dq pvc.
+
+Definition statefulset_replicas sts : nat :=
+  match sts.(StatefulSetV.Spec').(StatefulSetSpecV.Replicas') with
+  | Some replicas => sint.nat replicas
+  | None => 1%nat
+  end.
+
+Definition desired_ordinals sts : list nat :=
+  seq 0 (statefulset_replicas sts).
+
+Definition pvc_claim_template_names sts : list go_string :=
+  (λ claim_template,
+    claim_template.(PersistentVolumeClaimV.ObjectMeta').(ObjectMetaV.Name'))
+  <$> sts.(StatefulSetV.Spec').(StatefulSetSpecV.VolumeClaimTemplates').
+
+Definition desired_pvc_name sts claim_template_name ordinal : go_string :=
+  claim_template_name ++ "-"%go ++
+  sts.(StatefulSetV.ObjectMeta').(ObjectMetaV.Name') ++ "-"%go ++
+  decimal_string ordinal.
+
+Definition desired_pvc_key sts claim_template_name ordinal : KKey.t := {|
+  KKey.Kind' := PersistentVolumeClaimV.kind;
+  KKey.Namespace' := sts.(StatefulSetV.ObjectMeta').(ObjectMetaV.Namespace');
+  KKey.Name' := desired_pvc_name sts claim_template_name ordinal;
+|}.
+
+Definition desired_pvc_key_candidates sts : list KKey.t :=
+  concat (
+    (λ ordinal,
+      (λ claim_template_name, desired_pvc_key sts claim_template_name ordinal)
+      <$> pvc_claim_template_names sts)
+    <$> desired_ordinals sts
+  ).
+
+(* The official StatefulSet controller stores PVC requirements in maps keyed by
+   template name, so duplicate claim-template names collapse to one object key. *)
+Definition desired_pvc_keys sts : list KKey.t :=
+  elements (list_to_set (C:=gset KKey.t) (desired_pvc_key_candidates sts)).
+
+Lemma desired_pvc_keys_no_dup sts : NoDup (desired_pvc_keys sts).
+Proof.
+  unfold desired_pvc_keys.
+  apply NoDup_elements.
+Qed.
+
+Definition missing_pvc_keys sts (pvcs : list PersistentVolumeClaimV.t) : list KKey.t :=
+  filter (λ key, key ∉ (PersistentVolumeClaimV.key <$> pvcs)) (desired_pvc_keys sts).
+
+Definition pvcs_match sts pvcs : Prop :=
+  PersistentVolumeClaimV.key <$> pvcs ≡ₚ desired_pvc_keys sts.
+
+Definition desired_pod_name sts ordinal : go_string :=
+  sts.(StatefulSetV.ObjectMeta').(ObjectMetaV.Name') ++ "-"%go ++ decimal_string ordinal.
+
+(* TODO: complete this definition *)
+Parameter pod_match : StatefulSetV.t → PodV.t → Prop.
+Axiom pod_match_decision : ∀ sts pod, Decision (pod_match sts pod).
+#[local] Existing Instance pod_match_decision.
+
+Definition desired_pod_key sts ordinal : KKey.t := {|
+  KKey.Kind' := PodV.kind;
+  KKey.Namespace' := sts.(StatefulSetV.ObjectMeta').(ObjectMetaV.Namespace');
+  KKey.Name' := desired_pod_name sts ordinal;
+|}.
+
+Definition desired_pod_keys sts : list KKey.t :=
+  desired_pod_key sts <$> desired_ordinals sts.
+
+Definition pod_has_member_name sts pod : Prop :=
+  ∃ ordinal,
+    pod.(PodV.ObjectMeta').(ObjectMetaV.Name') = desired_pod_name sts ordinal.
+
+Definition pod_has_member_key sts pod : Prop :=
+  ∃ ordinal, PodV.key pod = desired_pod_key sts ordinal.
+
+Definition member_name_prefix sts : go_string :=
+  sts.(StatefulSetV.ObjectMeta').(ObjectMetaV.Name') ++ "-"%go.
+
+Definition parse_member_name sts pod : option nat :=
+  match New.proof.string.prefix_suffix.strip_prefix (member_name_prefix sts)
+      (pod.(PodV.ObjectMeta').(ObjectMetaV.Name')) with
+  | Some suffix => parse_canonical_decimal_string suffix
+  | None => None
+  end.
+
+Lemma parse_member_name_sound sts pod ordinal :
+  parse_member_name sts pod = Some ordinal →
+  pod.(PodV.ObjectMeta').(ObjectMetaV.Name') = desired_pod_name sts ordinal.
+Proof.
+  unfold parse_member_name.
+  destruct (New.proof.string.prefix_suffix.strip_prefix (member_name_prefix sts)
+    (pod.(PodV.ObjectMeta').(ObjectMetaV.Name'))) as [suffix|] eqn:Hstrip; [|done].
+  intros Hparse.
+  apply parse_canonical_decimal_string_sound in Hparse.
+  apply New.proof.string.prefix_suffix.strip_prefix_correct in Hstrip.
+  unfold desired_pod_name, member_name_prefix in *.
+  rewrite Hstrip.
+  rewrite -Hparse.
+  by rewrite List.app_assoc.
+Qed.
+
+Lemma parse_member_name_complete sts pod ordinal :
+  pod.(PodV.ObjectMeta').(ObjectMetaV.Name') = desired_pod_name sts ordinal →
+  parse_member_name sts pod = Some ordinal.
+Proof.
+  intros Hname.
+  unfold parse_member_name.
+  rewrite Hname.
+  unfold desired_pod_name, member_name_prefix.
+  rewrite List.app_assoc.
+  rewrite New.proof.string.prefix_suffix.strip_prefix_complete.
+  apply parse_canonical_decimal_string_decimal_string.
+Qed.
+
+#[local] Instance pod_has_member_name_decision sts pod :
+  Decision (pod_has_member_name sts pod).
+Proof.
+  destruct (parse_member_name sts pod) as [ordinal|] eqn:Hparse.
+  - left. exists ordinal. by apply parse_member_name_sound.
+  - right. intros [ordinal Hname].
+    apply parse_member_name_complete in Hname.
+    congruence.
+Defined.
+
+Lemma pod_has_member_key_iff sts pod :
+  pod_has_member_key sts pod ↔
+  pod.(PodV.ObjectMeta').(ObjectMetaV.Namespace') =
+    sts.(StatefulSetV.ObjectMeta').(ObjectMetaV.Namespace') ∧
+  pod_has_member_name sts pod.
+Proof.
+  split.
+  - intros [ordinal Hkey].
+    split.
+    + apply (f_equal KKey.Namespace') in Hkey. exact Hkey.
+    + exists ordinal.
+      apply (f_equal KKey.Name') in Hkey. exact Hkey.
+  - intros [Hnamespace [ordinal Hname]].
+    exists ordinal.
+    unfold PodV.key, PodV.meta_key, desired_pod_key.
+    simpl. by rewrite Hnamespace Hname.
+Qed.
+
+#[local] Instance pod_has_member_key_decision sts pod :
+  Decision (pod_has_member_key sts pod).
+Proof.
+  destruct (decide (
+    pod.(PodV.ObjectMeta').(ObjectMetaV.Namespace') =
+      sts.(StatefulSetV.ObjectMeta').(ObjectMetaV.Namespace') ∧
+    pod_has_member_name sts pod)) as [Hmember|Hnot_member].
+  - left. by apply pod_has_member_key_iff.
+  - right. intros Hmember_key.
+    apply Hnot_member. by apply pod_has_member_key_iff.
+Defined.
+
+Example pod_has_member_name_accepts_one sts pod :
+  pod.(PodV.ObjectMeta').(ObjectMetaV.Name') =
+    sts.(StatefulSetV.ObjectMeta').(ObjectMetaV.Name') ++ "-1"%go →
+  pod_has_member_name sts pod.
+Proof.
+  intros Hname.
+  exists 1%nat.
+  unfold desired_pod_name, decimal_string.
+  simpl.
+  exact Hname.
+Qed.
+
+Example pod_has_member_name_rejects_leading_zero sts pod :
+  pod.(PodV.ObjectMeta').(ObjectMetaV.Name') =
+    sts.(StatefulSetV.ObjectMeta').(ObjectMetaV.Name') ++ "-01"%go →
+  ¬ pod_has_member_name sts pod.
+Proof.
+  intros Hname [ordinal Hmember].
+  pose proof (parse_member_name_complete sts pod ordinal Hmember) as Hparse.
+  unfold parse_member_name, member_name_prefix in Hparse.
+  rewrite Hname in Hparse.
+  replace (sts.(StatefulSetV.ObjectMeta').(ObjectMetaV.Name') ++ "-01"%go)
+    with ((sts.(StatefulSetV.ObjectMeta').(ObjectMetaV.Name') ++ "-"%go) ++ "01"%go)
+    in Hparse by (rewrite -List.app_assoc; done).
+  rewrite New.proof.string.prefix_suffix.strip_prefix_complete in Hparse.
+  simpl in Hparse. done.
+Qed.
+
+Definition pod_key_is_desired sts key : Prop :=
+  key ∈ desired_pod_keys sts.
+
+#[local] Instance pod_key_is_desired_decision sts key :
+    Decision (pod_key_is_desired sts key).
+Proof. unfold pod_key_is_desired. apply _. Defined.
+
+Lemma desired_pod_key_inj sts : Inj (=) (=) (desired_pod_key sts).
+Proof.
+  intros ordinal1 ordinal2 Hkey.
+  apply (f_equal KKey.Name') in Hkey.
+  simpl in Hkey.
+  unfold desired_pod_name in Hkey.
+  apply app_inv_head in Hkey.
+  apply app_inv_head in Hkey.
+  by apply decimal_string_inj in Hkey.
+Qed.
+
+Lemma desired_pod_keys_no_dup sts : NoDup (desired_pod_keys sts).
+Proof.
+  unfold desired_pod_keys, desired_ordinals.
+  apply NoDup_fmap_2.
+  - apply desired_pod_key_inj.
+  - apply NoDup_seq.
+Qed.
+
+Definition missing_pod_keys sts (pods : list PodV.t) : list KKey.t :=
+  filter (λ key, key ∉ (PodV.key <$> pods)) (desired_pod_keys sts).
+
+Definition needed_pods sts pods : list PodV.t :=
+  filter (λ pod, pod_key_is_desired sts (PodV.key pod)) pods.
+
+Definition outdated_pods sts pods : list PodV.t :=
+  filter (λ pod, ¬ pod_match sts pod) (needed_pods sts pods).
+
+Definition bad_name_pods sts pods : list PodV.t :=
+  filter (λ pod, ¬ pod_has_member_key sts pod) pods.
+
+Definition alive_condemned_pods sts pods : list PodV.t :=
+  filter
+    (λ pod, pod_has_member_key sts pod ∧ ¬ pod_key_is_desired sts (PodV.key pod) ∧
+      is_pod_alive pod)
+    pods.
+
+(* The progress metric gives an outdated desired Pod cost 2 and a missing
+   desired Pod cost 1, so deleting one outdated Pod strictly reduces the
+   distance even though the desired replacement Pod is created by a later run. *)
+Definition pod_distance sts pods : nat :=
+  length (missing_pod_keys sts pods) +
+  2 * length (outdated_pods sts pods) +
+  length (bad_name_pods sts pods) +
+  length (alive_condemned_pods sts pods).
+
+Definition undesired_pvc_keys sts pvcs : list KKey.t :=
+  filter (λ key, key ∉ desired_pvc_keys sts) (PersistentVolumeClaimV.key <$> pvcs).
+
+Definition pvc_distance sts pvcs : nat :=
+  length (missing_pvc_keys sts pvcs) + length (undesired_pvc_keys sts pvcs).
+
+Definition match_distance sts pods pvcs : nat :=
+  pod_distance sts pods + pvc_distance sts pvcs.
+
+Definition pods_match sts pods : Prop :=
+  Forall (pod_has_member_key sts) pods ∧
+  Forall (λ pod, ¬ pod_key_is_desired sts (PodV.key pod) → ¬ is_pod_alive pod) pods ∧
+  PodV.key <$> needed_pods sts pods ≡ₚ desired_pod_keys sts ∧
+  Forall (pod_match sts) (needed_pods sts pods).
+
+Definition current_state_matches sts pods pvcs : Prop :=
+  pods_match sts pods ∧ pvcs_match sts pvcs.
+
+Lemma own_pods_frags_no_dup γ pods :
+  own_pods_frags γ 1 pods -∗
+  ⌜ NoDup (PodV.key <$> pods) ⌝.
+Proof.
+  iIntros "Hpods".
+  iAssert ([∗ list] pod ∈ pods,
+      own_meta_frag γ (PodV.key pod)
+        pod.(PodV.ObjectMeta').(ObjectMetaV.UID') 1 pod.(PodV.ObjectMeta'))%I
+    with "[Hpods]" as "Hpod_meta_frags".
+  { unfold own_pods_frags, own_pod_frags.
+    iInduction pods as [|pod pods] "IH".
+    - rewrite !big_sepL_nil. done.
+    - rewrite !big_sepL_cons.
+      iDestruct "Hpods" as "[(Hmeta & _) Hpods]".
+      iFrame "Hmeta".
+      iApply ("IH" with "Hpods"). }
+  iPoseProof (kview.own_meta_list_no_dup PodV.key PodV.ObjectMeta'
+    with "Hpod_meta_frags") as "%Hnodup".
+  done.
+Qed.
+
+Lemma own_pvcs_frags_no_dup γ pvcs :
+  own_pvcs_frags γ 1 pvcs -∗
+  ⌜ NoDup (PersistentVolumeClaimV.key <$> pvcs) ⌝.
+Proof.
+  iIntros "Hpvcs".
+  iAssert ([∗ list] pvc ∈ pvcs,
+      own_meta_frag γ (PersistentVolumeClaimV.key pvc)
+        pvc.(PersistentVolumeClaimV.ObjectMeta').(ObjectMetaV.UID') 1
+        pvc.(PersistentVolumeClaimV.ObjectMeta'))%I
+    with "[Hpvcs]" as "Hpvc_meta_frags".
+  { unfold own_pvcs_frags, own_pvc_frags.
+    iInduction pvcs as [|pvc pvcs] "IH".
+    - rewrite !big_sepL_nil. done.
+    - rewrite !big_sepL_cons.
+      iDestruct "Hpvcs" as "[(Hmeta & _) Hpvcs]".
+      iFrame "Hmeta".
+      iApply ("IH" with "Hpvcs"). }
+  iPoseProof (kview.own_meta_list_no_dup
+    PersistentVolumeClaimV.key PersistentVolumeClaimV.ObjectMeta'
+    with "Hpvc_meta_frags") as "%Hnodup".
+  done.
+Qed.
+
+Lemma match_distance_zero_matches γ sts pods pvcs :
+  own_pods_frags γ 1 pods -∗
+  own_pvcs_frags γ 1 pvcs -∗
+  ⌜ match_distance sts pods pvcs = 0%nat ↔ current_state_matches sts pods pvcs ⌝.
+Proof.
+  iIntros "Hpods Hpvcs".
+  iPoseProof (own_pods_frags_no_dup with "Hpods") as "%Hpods_nodup".
+  iPoseProof (own_pvcs_frags_no_dup with "Hpvcs") as "%Hpvcs_nodup".
+  iPureIntro.
+  pose proof (desired_pod_keys_no_dup sts) as Hdesired_pods_nodup.
+  pose proof (desired_pvc_keys_no_dup sts) as Hdesired_pvcs_nodup.
+  split.
+  - intros Hdist.
+    unfold match_distance, pod_distance, pvc_distance in Hdist.
+    assert (Hmissing_pods : length (missing_pod_keys sts pods) = 0%nat) by lia.
+    assert (Houtdated_pods : length (outdated_pods sts pods) = 0%nat) by lia.
+    assert (Hbad_name_pods : length (bad_name_pods sts pods) = 0%nat) by lia.
+    assert (Halive_condemned_pods :
+        length (alive_condemned_pods sts pods) = 0%nat) by lia.
+    assert (Hmissing_pvcs : length (missing_pvc_keys sts pvcs) = 0%nat) by lia.
+    assert (Hundesired_pvcs : length (undesired_pvc_keys sts pvcs) = 0%nat) by lia.
+    assert (Hpod_good_name : ∀ pod,
+        pod ∈ pods → pod_has_member_key sts pod).
+    { intros pod Hpod.
+      destruct (decide (pod_has_member_key sts pod)) as [Hgood|Hbad]; [done|].
+      exfalso.
+      eapply (filter_length_zero_not_elem
+        (λ pod, ¬ pod_has_member_key sts pod) pods pod);
+        [exact Hbad_name_pods|exact Hpod|exact Hbad]. }
+    assert (Hdesired_pod_actual : ∀ key,
+        key ∈ desired_pod_keys sts → key ∈ PodV.key <$> pods).
+    { intros key Hdesired.
+      destruct (decide (key ∈ PodV.key <$> pods)) as [Hactual|Hnot_actual]; [done|].
+      exfalso.
+      eapply (filter_length_zero_not_elem
+        (λ key, key ∉ (PodV.key <$> pods)) (desired_pod_keys sts) key);
+        [exact Hmissing_pods|exact Hdesired|exact Hnot_actual]. }
+    split.
+    + split.
+      * apply Forall_forall. intros pod Hpod.
+        rewrite <- list_elem_of_In in Hpod.
+        by apply Hpod_good_name.
+      * split.
+        -- apply Forall_forall. intros pod Hpod Hnot_desired Halive.
+           rewrite <- list_elem_of_In in Hpod.
+           eapply (filter_length_zero_not_elem
+             (λ pod, pod_has_member_key sts pod ∧ ¬ pod_key_is_desired sts (PodV.key pod) ∧
+               is_pod_alive pod)
+             pods pod);
+             [exact Halive_condemned_pods|exact Hpod|].
+           repeat split; [by apply Hpod_good_name|exact Hnot_desired|exact Halive].
+        -- split.
+           ++ apply NoDup_Permutation.
+              ** apply NoDup_fmap_filter. exact Hpods_nodup.
+              ** exact Hdesired_pods_nodup.
+              ** intros key. split.
+                 --- intros Hactual.
+                     apply list_elem_of_fmap_1 in Hactual as (pod & Hkey_eq & Hpod_filter).
+                     apply list_elem_of_filter in Hpod_filter as [Hpod_desired _].
+                     unfold pod_key_is_desired in Hpod_desired.
+                     rewrite Hkey_eq. exact Hpod_desired.
+                 --- intros Hdesired.
+                     apply Hdesired_pod_actual in Hdesired as Hactual.
+                     apply list_elem_of_fmap_1 in Hactual as (pod & Hkey_eq & Hpod).
+                     rewrite Hkey_eq.
+                     apply list_elem_of_fmap_2.
+                     apply list_elem_of_filter.
+                     split; [|exact Hpod].
+                     unfold pod_key_is_desired.
+                     rewrite -Hkey_eq. exact Hdesired.
+           ++ apply Forall_forall. intros pod Hpod.
+              rewrite <- list_elem_of_In in Hpod.
+              assert (Hpod_needed : pod ∈ needed_pods sts pods) by exact Hpod.
+              unfold needed_pods in Hpod.
+              apply list_elem_of_filter in Hpod as [Hpod_desired Hpod].
+              destruct (decide (pod_match sts pod)) as [Hmatch|Hnot_match]; [exact Hmatch|].
+              exfalso.
+              eapply (filter_length_zero_not_elem
+                (λ pod, ¬ pod_match sts pod)
+                (needed_pods sts pods) pod);
+                [|exact Hpod_needed|exact Hnot_match].
+              unfold outdated_pods in Houtdated_pods. exact Houtdated_pods.
+    + apply NoDup_Permutation; [exact Hpvcs_nodup|exact Hdesired_pvcs_nodup|].
+      intros key. split.
+      * intros Hactual.
+        destruct (decide (key ∈ desired_pvc_keys sts)) as [Hdesired|Hnot_desired]; [done|].
+        exfalso.
+        eapply (filter_length_zero_not_elem
+          (λ key, key ∉ desired_pvc_keys sts) (PersistentVolumeClaimV.key <$> pvcs) key);
+          [exact Hundesired_pvcs|exact Hactual|exact Hnot_desired].
+      * intros Hdesired.
+        destruct (decide (key ∈ PersistentVolumeClaimV.key <$> pvcs)) as [Hactual|Hnot_actual]; [done|].
+        exfalso.
+        eapply (filter_length_zero_not_elem
+          (λ key, key ∉ (PersistentVolumeClaimV.key <$> pvcs)) (desired_pvc_keys sts) key);
+          [exact Hmissing_pvcs|exact Hdesired|exact Hnot_actual].
+  - intros [[Hmember [Hcondemned [Hneeded_perm Hneeded_match]]] Hpvcs_perm].
+    unfold match_distance, pod_distance, pvc_distance.
+    assert (Hmissing_pods_nil : missing_pod_keys sts pods = []).
+    { unfold missing_pod_keys.
+      apply filter_none. intros key Hdesired Hnot_actual.
+      apply Hnot_actual.
+      rewrite -Hneeded_perm in Hdesired.
+      apply list_elem_of_fmap_1 in Hdesired as (pod & Hkey_eq & Hpod_needed).
+      rewrite Hkey_eq. apply list_elem_of_fmap_2.
+      unfold needed_pods in Hpod_needed.
+      apply list_elem_of_filter in Hpod_needed as [_ Hpod].
+      exact Hpod. }
+    assert (Houtdated_pods_nil : outdated_pods sts pods = []).
+    { unfold outdated_pods.
+      apply filter_none. intros pod Hpod Hnot_match.
+      rewrite Forall_forall in Hneeded_match.
+      rewrite list_elem_of_In in Hpod.
+      exact (Hnot_match (Hneeded_match pod Hpod)). }
+    assert (Hbad_name_pods_nil : bad_name_pods sts pods = []).
+    { unfold bad_name_pods.
+      apply filter_none. intros pod Hpod Hnot_member.
+      rewrite Forall_forall in Hmember.
+      rewrite list_elem_of_In in Hpod.
+      exact (Hnot_member (Hmember pod Hpod)). }
+    assert (Halive_condemned_pods_nil : alive_condemned_pods sts pods = []).
+    { unfold alive_condemned_pods.
+      apply filter_none. intros pod Hpod (_ & Hnot_desired & Halive).
+      rewrite Forall_forall in Hcondemned.
+      rewrite list_elem_of_In in Hpod.
+      exact (Hcondemned pod Hpod Hnot_desired Halive). }
+    assert (Hmissing_pvcs_nil : missing_pvc_keys sts pvcs = []).
+    { unfold missing_pvc_keys.
+      apply filter_none. intros key Hdesired Hnot_actual.
+      apply Hnot_actual. by rewrite Hpvcs_perm. }
+    assert (Hundesired_pvcs_nil : undesired_pvc_keys sts pvcs = []).
+    { unfold undesired_pvc_keys.
+      apply filter_none. intros key Hactual Hnot_desired.
+      apply Hnot_desired. by rewrite -Hpvcs_perm. }
+    rewrite Hmissing_pods_nil Houtdated_pods_nil Hbad_name_pods_nil
+      Halive_condemned_pods_nil Hmissing_pvcs_nil Hundesired_pvcs_nil.
+    done.
+Qed.
+
+Lemma wp_syncStatefulSet_progress γ l (gv: schema.GroupVersion.t) namespace name sts dq pods pvcs :
+  {{{ is_pkg_init code.controllers.statefulset.pkg_id.statefulset ∗
+      "#Hisk" ∷ is_kubernetes γ l ∗
+      "#Hglobal_l" ∷ (global_addr apimodel.ModelState) ↦□ l ∗
+      "#Hglobal_gv" ∷ (global_addr apps_v1.SchemeGroupVersion) ↦□ gv ∗
+      "Hown_sts_meta_frag" ∷ own_meta_frag γ (StatefulSetV.key sts) sts.(StatefulSetV.ObjectMeta').(ObjectMetaV.UID') dq sts.(StatefulSetV.ObjectMeta') ∗
+      "Hown_sts_spec_frag" ∷ own_spec_frag γ (StatefulSetV.key sts) sts.(StatefulSetV.ObjectMeta').(ObjectMetaV.UID') dq (ObjectSpecV.StatefulSetSpec sts.(StatefulSetV.Spec')) ∗
+      "Hown_pod_frags" ∷ own_pods_frags γ 1 pods ∗
+      "Hown_pvc_frags" ∷ own_pvcs_frags γ 1 pvcs ∗
+      "Hown_children_frag" ∷ own_children_frag γ (StatefulSetV.key sts) sts.(StatefulSetV.ObjectMeta').(ObjectMetaV.UID') 1 (list_to_set (PodV.key <$> pods)) ∗
+      "Hown_reserved_missing_pod_keys" ∷ ([∗ list] key ∈ missing_pod_keys sts pods, own_reserved_frag γ key) ∗
+      "Hown_reserved_missing_pvc_keys" ∷ ([∗ list] key ∈ missing_pvc_keys sts pvcs, own_reserved_frag γ key) ∗
+      "%Hnamespace_eq" ∷ ⌜ namespace = sts.(StatefulSetV.ObjectMeta').(ObjectMetaV.Namespace') ⌝ ∗
+      "%Hname_eq" ∷ ⌜ name = sts.(StatefulSetV.ObjectMeta').(ObjectMetaV.Name') ⌝ ∗
+      "%Hdeletion_timestamp_eq" ∷ ⌜ sts.(StatefulSetV.ObjectMeta').(ObjectMetaV.DeletionTimestamp') = None ⌝ ∗
+      "%Hnot_match" ∷ ⌜ ¬ current_state_matches sts pods pvcs ⌝
+  }}}
+    @! statefulset.syncStatefulSet #namespace #name
+  {{{ (pods' : list PodV.t) (pvcs' : list PersistentVolumeClaimV.t) (err : interface.t), RET #err;
+      ((⌜ err = interface.nil ⌝ ∗ ⌜ current_state_matches sts pods' pvcs' ⌝) ∨
+       (⌜ err ≠ interface.nil ⌝ ∗ ⌜ match_distance sts pods pvcs > match_distance sts pods' pvcs' ⌝)) ∗
+      own_meta_frag γ (StatefulSetV.key sts) sts.(StatefulSetV.ObjectMeta').(ObjectMetaV.UID') dq sts.(StatefulSetV.ObjectMeta') ∗
+      own_spec_frag γ (StatefulSetV.key sts) sts.(StatefulSetV.ObjectMeta').(ObjectMetaV.UID') dq (ObjectSpecV.StatefulSetSpec sts.(StatefulSetV.Spec')) ∗
+      own_pods_frags γ 1 pods' ∗
+      own_pvcs_frags γ 1 pvcs' ∗
+      own_children_frag γ (StatefulSetV.key sts) sts.(StatefulSetV.ObjectMeta').(ObjectMetaV.UID') 1 (list_to_set (PodV.key <$> pods'))
+  }}}.
+Proof.
+Admitted.
+
+Lemma wp_syncStatefulSet_stability γ l (gv: schema.GroupVersion.t) namespace name sts dq pods pvcs :
+  {{{ is_pkg_init code.controllers.statefulset.pkg_id.statefulset ∗
+      "#Hisk" ∷ is_kubernetes γ l ∗
+      "#Hglobal_l" ∷ (global_addr apimodel.ModelState) ↦□ l ∗
+      "#Hglobal_gv" ∷ (global_addr apps_v1.SchemeGroupVersion) ↦□ gv ∗
+      "Hown_sts_meta_frag" ∷ own_meta_frag γ (StatefulSetV.key sts) sts.(StatefulSetV.ObjectMeta').(ObjectMetaV.UID') dq sts.(StatefulSetV.ObjectMeta') ∗
+      "Hown_sts_spec_frag" ∷ own_spec_frag γ (StatefulSetV.key sts) sts.(StatefulSetV.ObjectMeta').(ObjectMetaV.UID') dq (ObjectSpecV.StatefulSetSpec sts.(StatefulSetV.Spec')) ∗
+      "Hown_pod_frags" ∷ own_pods_frags γ dq pods ∗
+      "Hown_pvc_frags" ∷ own_pvcs_frags γ dq pvcs ∗
+      "Hown_children_frag" ∷ own_children_frag γ (StatefulSetV.key sts) sts.(StatefulSetV.ObjectMeta').(ObjectMetaV.UID') dq (list_to_set (PodV.key <$> pods)) ∗
+      "Hown_reserved_missing_pod_keys" ∷ ([∗ list] key ∈ missing_pod_keys sts pods, own_reserved_frag γ key) ∗
+      "Hown_reserved_missing_pvc_keys" ∷ ([∗ list] key ∈ missing_pvc_keys sts pvcs, own_reserved_frag γ key) ∗
+      "%Hnamespace_eq" ∷ ⌜ namespace = sts.(StatefulSetV.ObjectMeta').(ObjectMetaV.Namespace') ⌝ ∗
+      "%Hname_eq" ∷ ⌜ name = sts.(StatefulSetV.ObjectMeta').(ObjectMetaV.Name') ⌝ ∗
+      "%Hdeletion_timestamp_eq" ∷ ⌜ sts.(StatefulSetV.ObjectMeta').(ObjectMetaV.DeletionTimestamp') = None ⌝ ∗
+      "%Hnot_match" ∷ ⌜ current_state_matches sts pods pvcs ⌝
+  }}}
+    @! statefulset.syncStatefulSet #namespace #name
+  {{{ RET #interface.nil;
+      own_meta_frag γ (StatefulSetV.key sts) sts.(StatefulSetV.ObjectMeta').(ObjectMetaV.UID') dq sts.(StatefulSetV.ObjectMeta') ∗
+      own_spec_frag γ (StatefulSetV.key sts) sts.(StatefulSetV.ObjectMeta').(ObjectMetaV.UID') dq (ObjectSpecV.StatefulSetSpec sts.(StatefulSetV.Spec')) ∗
+      own_pods_frags γ dq pods ∗
+      own_pvcs_frags γ dq pvcs ∗
+      own_children_frag γ (StatefulSetV.key sts) sts.(StatefulSetV.ObjectMeta').(ObjectMetaV.UID') dq (list_to_set (PodV.key <$> pods))
+  }}}.
+Proof.
+Admitted.
+
+End proof.
